wip

mem/Mem01proof.v
@@ -18,8 +18,6 @@ From ExtLib Require Import
 Require Import TODOYJ.
 Require Import HTactics Logic YPM.
 
-Generalizable Variables E R A B C X Y.
-
 Set Implicit Arguments.
 
 Local Open Scope nat_scope.
@@ -146,33 +144,429 @@ Proof. ii. subst. unfold dec. destruct H; ss. Qed.
 (*   - *)
 (* Qed. *)
 
+
+Module PARSE.
+  Section PARSE.
+    Context `{Σ: GRA.t}.
+
+    Inductive iProp_tree: Type :=
+    | iProp_tree_base (P: iProp)
+    | iProp_tree_binop (op: iProp -> iProp -> iProp) (tr0 tr1: iProp_tree)
+    | iProp_tree_unop (op: iProp -> iProp) (tr: iProp_tree)
+    | iProp_tree_kop A (op: (A -> iProp) -> iProp) (k: A -> iProp_tree)
+    .
+
+    Fixpoint from_iProp_tree (tr: iProp_tree): iProp :=
+      match tr with
+      | iProp_tree_base P => P
+      | iProp_tree_binop op P Q => op (from_iProp_tree P) (from_iProp_tree Q)
+      | iProp_tree_unop op P => op (from_iProp_tree P)
+      | @iProp_tree_kop A op k => op (fun a => from_iProp_tree (k a))
+      end.
+
+    Definition hole (A: Type): A. Admitted.
+
+    Ltac parse_iProp_tree p :=
+      match p with
+      | ?op (?P0: iProp) (?P1: iProp) =>
+        let tr0 := parse_iProp_tree P0 in
+        let tr1 := parse_iProp_tree P1 in
+        constr:(iProp_tree_binop op tr0 tr1)
+      | ?op (?P: iProp) =>
+        let tr := parse_iProp_tree P in
+        constr:(iProp_tree_unop op tr)
+      | ?op ?k =>
+        match type of k with
+        | ?A -> bi_car iProp =>
+          let khole := (eval cbn beta in (k (@hole A))) in
+          let tr := parse_iProp_tree khole in
+          let fhole := (eval pattern (@hole A) in tr) in
+          match fhole with
+          | ?f (@hole A) => constr:(@iProp_tree_kop A op f)
+          end
+        end
+      | ?P => constr:(iProp_tree_base P)
+      end.
+
+    Definition iProp_list := alist string iProp_tree.
+
+    Definition from_iProp_list (l: iProp_list): iProp :=
+      fold_alist (fun _ tr acc => from_iProp_tree tr ** acc) (emp)%I l.
+  End PARSE.
+End PARSE.
+
+
+Section ALIST.
+  Fixpoint alist_pop (K : Type) (R : K → K → Prop) (RD_K : RelDec R) (V : Type)
+           (k : K) (m : alist K V): option (V * alist K V) :=
+    match m with
+    | [] => None
+    | (k', v) :: ms =>
+      if k ?[R] k'
+      then Some (v, ms)
+      else match @alist_pop K R RD_K V k ms with
+           | Some (v', ms') => Some (v', (k', v) :: ms')
+           | None => None
+           end
+    end.
+
+End ALIST.
+Arguments alist_pop [K R] {RD_K} [V].
+Arguments alist_remove [K R] {RD_K} [V].
+
+Section ILIST.
+  Context `{Σ: GRA.t}.
+
+  Definition iPropL := alist string iProp.
+
+  Definition from_iPropL (l: iPropL): iProp :=
+    fold_alist (fun _ P acc => P ** acc) (emp)%I l.
+
+  Definition iPropL_merge (Hn0 Hn1: string) (Hn2: string) (l0: iPropL): option iPropL :=
+    do '(P0, l1) <- alist_pop Hn0 l0;
+    do '(P1, l2) <- alist_pop Hn1 l1;
+    Some (alist_add Hn0
+
+                    destruct *
+          make pure
+               destruct ex
+               assert
+          /\
+          destruct \/
+          upd
+
+  Definition Sepconj (P Q: iProp'): iProp' :=
+    Seal.sealing
+      "iProp"
+      (fun r => exists a b, r = URA.add a b /\ P a /\ Q b).
+  Definition Pure (P: Prop): iProp' :=
+    Seal.sealing
+      "iProp"
+      (fun _ => P).
+  Definition Ex {X: Type} (P: X -> iProp'): iProp' :=
+    Seal.sealing
+      "iProp"
+      (fun r => exists x, P x r).
+  Definition Univ {X: Type} (P: X -> iProp'): iProp' :=
+    Seal.sealing
+      "iProp"
+      (fun r => forall x, P x r).
+  Definition Own (r0: Σ): iProp' :=
+    Seal.sealing
+      "iProp"
+      (fun r1 => URA.extends r0 r1).
+  Definition And (P Q: iProp'): iProp' :=
+    Seal.sealing
+      "iProp"
+      (fun r => P r /\ Q r).
+  Definition Or (P Q: iProp'): iProp' :=
+    Seal.sealing
+      "iProp"
+      (fun r => P r \/ Q r).
+  Definition Impl (P Q: iProp'): iProp' :=
+    Seal.sealing
+      "iProp"
+      (fun r => URA.wf r -> P r -> Q r).
+  Definition Wand (P Q: iProp'): iProp' :=
+    Seal.sealing
+      "iProp"
+      (fun r => forall rp, URA.wf (r ⋅ rp) -> P rp -> Q (r ⋅ rp)).
+  Definition Upd (P: iProp'): iProp' :=
+    Seal.sealing
+      "iProp"
+      (fun r0 => forall ctx, URA.wf (r0 ⋅ ctx) -> exists r1, URA.wf (r1 ⋅ ctx) /\ P r1).
+
+
+                    assert
+                    split
+                    pure
+                    destruct *
+          destruct \/
+          de
+
+    None.
+
+    match exprs with
+    | h :: t =>
+      do hexp <- (compile_expr h); compile_exprs t (acc ++ [hexp])
+    | [] => Some acc
+    end
+  .
+
+    alist_find
+
+
+
+
+  alist_update
+
+  Definiti
+
+  Definition from_iPropR
+
+  Lemma from_iPropL_split (Pn Qn: string) (P Q: iPropL)
+
+        (l0 ++ P :: l1)
+
+
+  Fixpoi
+
+  alist _add
+
+
+
+  Inductive iProp_tree: Type :=
+  | iProp_tree_base (P: iProp)
+  | iProp_tree_binop (op: iProp -> iProp -> iProp) (tr0 tr1: iProp_tree)
+  | iProp_tree_unop (op: iProp -> iProp) (tr: iProp_tree)
+  | iProp_tree_kop A (op: (A -> iProp) -> iProp) (k: A -> iProp_tree)
+  .
+
+  Fixpoint from_iProp_tree (tr: iProp_tree): iProp :=
+    match tr with
+    | iProp_tree_base P => P
+    | iProp_tree_binop op P Q => op (from_iProp_tree P) (from_iProp_tree Q)
+    | iProp_tree_unop op P => op (from_iProp_tree P)
+    | @iProp_tree_kop A op k => op (fun a => from_iProp_tree (k a))
+    end.
+
+  Definition hole (A: Type): A. Admitted.
+
+  Ltac parse_iProp_tree p :=
+    match p with
+    | ?op (?P0: iProp) (?P1: iProp) =>
+      let tr0 := parse_iProp_tree P0 in
+      let tr1 := parse_iProp_tree P1 in
+      constr:(iProp_tree_binop op tr0 tr1)
+    | ?op (?P: iProp) =>
+      let tr := parse_iProp_tree P in
+      constr:(iProp_tree_unop op tr)
+    | ?op ?k =>
+      match type of k with
+      | ?A -> bi_car iProp =>
+        let khole := (eval cbn beta in (k (@hole A))) in
+        let tr := parse_iProp_tree khole in
+        let fhole := (eval pattern (@hole A) in tr) in
+        match fhole with
+        | ?f (@hole A) => constr:(@iProp_tree_kop A op f)
+        end
+      end
+    | ?P => constr:(iProp_tree_base P)
+    end.
+
+  Definition iProp_list := alist string iProp_tree.
+
+  Definition from_iProp_list (l: iProp_list): iProp :=
+    fold_alist (fun _ tr acc => from_iProp_tree tr ** acc) (emp)%I l.
+End PARSE.
+End PARSE.
+
+
+alist_add
+
+
 Section SIMMODSEM.
 
   Context `{Σ: GRA.t}.
   Context `{@GRA.inG Mem1.memRA Σ}.
 
-  Let W: Type := ((Σ * Any.t)) * ((Σ * Any.t)).
   (* Eval compute in (@RA.car (RA.excl Mem.t)). *)
   Eval compute in (@URA.car Mem1._memRA).
   Inductive sim_loc: option val -> URA.car (t:=(Excl.t _)) -> Prop :=
   | sim_loc_present v: sim_loc (Some v) (Some v)
   | sim_loc_absent: sim_loc None ε
   .
+  Hint Constructors sim_loc: core.
 
+    Definition mem_tgt: Mem.t. Admitted.
+
+    Definition aa: iProp :=
+      ((⌜5 = 7⌝ ** ⌜9 = 10⌝)
+         **
+         (∃ mem_src, (Own (GRA.embed ((Auth.black mem_src): URA.car (t:=Mem1.memRA))))
+                       **
+                       (⌜forall b ofs, sim_loc ((mem_tgt.(Mem.cnts)) b ofs) (mem_src b ofs)⌝)))%I.
+
+    Definition cc: iProp :=
+      (∃ (n: nat), ⌜(n + 1 = 1 + n)%nat⌝)%I.
+
+    Goal bi_entails aa cc.
+    Proof.
+      unfold aa, cc.
+      match goal with
+      |  |- bi_entails ?a _ =>
+         let tr := parse_iProp_tree a in
+         change a with (from_iProp_tree tr)
+      end.
+      admit "".
+    Qed.
+
+    Admitted.
+      Show Proof.
+
+      let k := constr:(fun n: nat => ⌜(n = n)⌝ ** ⌜(n = n)⌝%I: iProp) in
+      (match type of k with
+       | ?A -> bi_car iProp =>
+         let khole := eval cbn beta in (k (@hole A)) in
+             let tr := parse_iProp_tree khole in
+             let fhole := eval pattern (@hole A) in tr in
+                 match fhole with
+                 | ?f (@hole A) => constr:(@iProp_tree_kop A bi_exist f)
+                 end
+       end).
+
+      let k := constr:(fun n: nat => ⌜(n = n)⌝ ** ⌜(n = n)⌝%I: iProp) in
+      (match type of k with
+       | ?A -> bi_car iProp =>
+         let khole := eval cbn beta in (k (@hole A)) in
+             let tr := parse_iProp_tree khole in
+             let a := pattern (@hole A) in tr in
+                 match a with
+                 | ?f (@hole A) => pose f
+                 end
+       end).
+
+
+
+           in
+
+             admit ""
+
+
+         uconstr:()
+
+         unshelve epose (_: A -> iProp_tree);
+         [
+           let tmp := fresh A in
+           intros tmp;
+           let kp := eval simpl in (k tmp) in
+               let tr := parse_iProp_tree kp in
+               exact tr
+         |
+         match goal with
+         | [ktr: A -> iProp_tree |- _] =>
+           match eval unfold ktr in ktr with
+           | ?v => clear ktr; pose (@iProp_tree_kop A bi_exist v)
+           end
+         end
+         ]
+       end).
+
+      ) with
+           | ?aaa => idtac
+             end
+             .
+
+      match (let k := constr:(fun n: nat => ⌜(n = n)⌝ ** ⌜(n = n)⌝%I: iProp) in
+             (match type of k with
+              | ?A -> bi_car iProp =>
+                unshelve epose (_: A -> iProp_tree);
+                [
+                  let tmp := fresh A in
+                  intros tmp;
+                  let kp := eval simpl in (k tmp) in
+                      let tr := parse_iProp_tree kp in
+                      exact tr
+                |
+                match goal with
+                | [ktr: A -> iProp_tree |- _] =>
+                  match eval unfold ktr in ktr with
+                  | ?v => clear ktr; pose (@iProp_tree_kop A bi_exist v); constr:(1)
+                  end
+                end
+                ]
+              end)) with
+      | ?aaa => idtac
+      end
+      .
+
+        in pose x.
+
+      Show Proof
+
+      unshelve epose (_: nat -> iProp_tree).
+      { intros n.
+        let tr := parse_iProp_tree constr:((fun n: nat => ⌜(n = n)⌝ ** ⌜(n = n)⌝%I: iProp) n) in pose tr.
+
+
+      clear i0.
+
+      Set Printing All.
+
+
+      clear i.
+      pose (fun n: nat => ⌜(n = n)⌝%I: iProp).
+
+      epose (_: nat). := _).
+
+      epose (_: nat -> iProp_tree).
+      { intros n.
+        match constr:(b n) with
+        | ?P =>
+          let tr := parse_iProp_tree P in
+          exact tr
+        end.
+      }
+
+        match (b with
+
+      unshelve eauto.
+
+
+      match constr:(fun n: nat => ⌜(n = n)⌝%I: iProp) with
+      | ?k =>
+        pose (fun n => k n)
+      end.
+
+      pose (fun n: nat => ⌜(n = n)⌝%I: iProp).
+
+
+      match goal with
+      |  |- bi_entails _ ?a =>
+
+         match a with
+         | ?op ?k =>
+           match type of k with
+           | ?A -> ?B =>
+             pose k
+           end
+         end
+      end.
+
+
+    Ltac parse_iProp_tree tr :=
+      match tr with
+      | ?op (?P0: iProp) (?P1: iProp) =>
+        let tr0 := parse_iProp_tree P0 in
+        let tr1 := parse_iProp_tree P1 in
+        constr:(iProp_tree_binop op tr0 tr1)
+      | ?op (?P: iProp) =>
+        let tr := parse_iProp_tree P in
+        constr:(iProp_tree_unop op tr)
+      | ?op (fun x => ?k x) =>
+        pose k;
+        let ktr := parse_iProp_tree (k x) in
+        constr:(iProp_tree_kop op (fun x => ktr))
+      | ?P => constr:(iProp_tree_base P)
+      end.
+
+
+      pose (parse_iProp
+
+      change aa with parse_i
+
+
+
+  Let W: Type := ((Σ * Any.t)) * ((Σ * Any.t)).
   Let wf: W -> Prop :=
-    fun '(mrps_src0, mrps_tgt0) =>
-      exists mr_src (mem_tgt: Mem.t),
-        (<<SRC: mrps_src0 = (mr_src, tt↑)>>) /\
-        (<<TGT: mrps_tgt0 = (ε, mem_tgt↑)>>) /\
-        (<<SIM: iHyp (Exists mem_src, Own (GRA.embed ((Auth.black mem_src): URA.car (t:=Mem1.memRA))) **
-                                          (* (Forall b ofs, ⌜~(b = 0 /\ ofs = 0%Z)⌝ -* *)
-                                          (*                  match mem_tgt.(Mem.cnts) b ofs with *)
-                                          (*                  | Some v => Own (GRA.embed ((b, ofs) |-> [v])) *)
-                                          (*                  | None => ⌜True⌝ *)
-                                          (*                  end) *)
-                                          (⌜forall b ofs, sim_loc ((mem_tgt.(Mem.cnts)) b ofs) (mem_src b ofs)⌝)
-                     ) mr_src>>) /\
-        (<<WFTGT: forall b ofs v, mem_tgt.(Mem.cnts) b ofs = Some v -> <<NB: b < mem_tgt.(Mem.nb)>> >>)
+    @mk_wf
+      _
+      Mem.t
+      (fun mem_tgt _ => (∃ mem_src, (Own (GRA.embed ((Auth.black mem_src): URA.car (t:=Mem1.memRA))))
+                                      **
+                                      (⌜forall b ofs, sim_loc ((mem_tgt.(Mem.cnts)) b ofs) (mem_src b ofs)⌝)
+                        )%I)
+      (fun mem_tgt mp_tgt _ => mp_tgt = mem_tgt↑ /\ forall b ofs v, mem_tgt.(Mem.cnts) b ofs = Some v -> <<NB: b < mem_tgt.(Mem.nb)>>)
   .
 
   Hint Resolve sim_itree_mon: paco.
@@ -185,29 +579,80 @@ Section SIMMODSEM.
   (* Opaque URA.pointwise. *)
   Opaque URA.unit.
 
+
+
+
+
+      ((⌜5 = 7⌝ ** ⌜9 = 10⌝) **
+                             (∃ mem_src : nat → Z → Excl.car,
+                                 (Own (GRA.embed ((Auth.black mem_src): URA.car (t:=Mem1.memRA)))) **
+                                                                                                   ⌜∀ (b : nat) (ofs : Z) (v: option val), sim_loc v (mem_src b ofs)⌝))%I.
+
+  End REFLECT.
+
   Theorem correct: ModPair.sim Mem1.Mem Mem0.Mem.
   Proof.
     econs; ss; [|admit "modsem wf"].
     i. eapply adequacy_lift.
     econstructor 1 with (wf:=wf); et; swap 2 3.
-    { ss. esplits; ss; et. hexploit gwf_dummy; i. iRefresh.
-      eexists; iRefresh. iSplitP; ss.
-      { eexists. rewrite URA.unit_id. refl. }
-      { ii. destruct (nth_error sk b) eqn:FIND.
-        { destruct p. cbn. des_ifs; try econs. }
-        { cbn. econs. }
+    { ss. red. econs; et; cycle 1.
+      { esplits; et. i. ss.
+        destruct (nth_error sk b) eqn:FIND; cbn in *; ss.
+        eapply nth_error_Some. ii. clarify.
       }
-      { i. ss. eapply nth_error_Some.
-        intros EQ. rewrite EQ in *. ss. }
+      { eapply to_semantic.
+        { iIntros "H". iExists _. iSplit.
+          { iApply "H". }
+          { iPureIntro. i. ss.
+            destruct (nth_error sk b) eqn:FIND; cbn in *; ss.
+            destruct p. des_ifs; econs.
+          }
+        }
+        { (* TODO: do we need to prove it? *)
+          eapply GRA.wf_embed. ur. split; auto.
+          { eexists. eapply URA.unit_idl. }
+          { ur. i. ur. i. ur. des_ifs. }
+        }
+      }
     }
-
     econs; ss.
     { unfold allocF. init.
-      harg_tac. des_ifs_safe. des. repeat rewrite URA.unit_idl in *. repeat rewrite URA.unit_id in *.
-      iRefresh. iPure PRE. des. clarify. apply Any.upcast_inj in PRE. des; clarify.
-      steps. rewrite Any.upcast_downcast in *. steps.
-      do 2 iDestruct SIM. iPure A.
-      set (blk := (Mem.nb mem_tgt)). rename x into sz. rename x0 into mem_src0.
+
+      (* harg_tac *)
+      eapply harg_clo; ss. clear SIMMRS mrs_src mrs_tgt.
+
+      i. des; clarify.
+
+      (* pure tac *)
+      exploit current_iprops_pure.
+      { eapply ACC. }
+
+
+      . in ACC; destruct ACC as [ACC PURE]; cycle 1.
+      { iIntros "[[H0 H1] _]". iCombine "H0 H1" as "H0". iApply "H0". }
+
+      des; clarify.
+
+      (* impl tac *)
+      eapply current_iprops_update in ACC; cycle 1.
+      { iIntros "[_ H2]". iApply "H2". }
+
+      (* exists tac *)
+      eapply current_iprops_exists in ACC; destruct ACC as [mem_src ACC].
+
+      (* pure tac *)
+      eapply current_iprops_pure in ACC; destruct ACC as [ACC PURE]; cycle 1.
+      { iIntros "[H0 H1]". iApply "H1". }
+
+      (* impl tac *)
+      eapply current_iprops_update in ACC; cycle 1.
+      { iIntros "[H0 _]". iApply "H0". }
+
+      steps. rewrite Any.upcast_downcast in *. steps. astart 0.
+      rename a into mem_tgt.
+      set (blk := (Mem.nb mem_tgt)).
+
+      rename x into sz. rename x0 into mem_src0.
 
       astart 0. astop.
 
